progress

Batteries/Data/BinomialHeap/Basic.lean
@@ -55,13 +55,13 @@ def HeapNode.rank : HeapNode α → Nat
   | .node _ _ s => s.rank + 1
 
 /-- Tail-recursive version of `HeapNode.rank`. -/
-@[inline] private def HeapNode.rankTR (s : HeapNode α) : Nat := go s 0 where
+@[inline] def HeapNode.rankTR (s : HeapNode α) : Nat := go s 0 where
   /-- Computes `s.rank + r` -/
   go : HeapNode α → Nat → Nat
   | .nil, r => r
   | .node _ _ s, r => go s (r + 1)
 
-@[csimp] private theorem HeapNode.rankTR_eq : @rankTR = @rank := by
+@[csimp] theorem HeapNode.rankTR_eq : @rankTR = @rank := by
   funext α s; exact go s 0
 where
   go {α} : ∀ s n, @rankTR.go α s n = rank s + n
